theories/Client.v
@@ -8,6 +8,7 @@ Require Import Monads.
 Require Import OCamlTypes.
 Require Import Recdef.
 Open Scope monad_scope.
+Open Scope sint63_scope.
 
 (**
     The internal loop of our client sending thread
@@ -15,9 +16,38 @@ Open Scope monad_scope.
 Definition client_send_thread (sockfd : file_descr) : optionE unit :=
     repeat_until_timeout max_int (fun _ => 
         let* _ <= print_string ">>> " #;
-        let msg := read_line tt in
-        _ <- send_message sockfd (serialize_client_message (MESG msg)) ;;
-        SomeE Recurse
+        msg <- read_line tt ;;
+        let* _ <= print_endline "read line" #;
+        match ((if (1 <? int_len_string msg) then
+            (* Check if a private message *)
+            let first_char := match get 0 msg with
+                              | Some a => a
+                              (* Not possible *)
+                              | None => space
+                              end in
+            if Ascii.eqb first_char ampersand then
+                (* First space splits username and message *)
+                let split_idx := match index 0 space_str msg with
+                                 | None => O
+                                 | Some n => n
+                                 end in
+                let msg_text :=
+                    substring (split_idx + 1) 
+                        (Z.to_nat (to_Z (int_len_string msg)) - split_idx) msg in
+                let uname_text :=
+                    substring 1 (split_idx - 1) msg in
+                uname <- new_username uname_text ;;
+                send_message sockfd (serialize_client_message (PMSG msg_text uname))
+            else
+                send_message sockfd (serialize_client_message 
+                    (MESG msg))
+        else
+            SomeE tt)) with
+        | SomeE _ => SomeE Recurse
+        | NoneE s => 
+            let* _ <= log Log_Error s #;
+            SomeE Recurse
+        end
     ).
 
 (**
@@ -30,6 +60,10 @@ Definition client_recv_thread (sockfd : file_descr) : optionE unit :=
         | MSG uname msg =>
             let* _ <= print_endline (uname.(Uname) ++ ": " ++ msg) #;
             print_string ">>> "
+        | ERR err =>
+            let* _ <= print_endline "" #;
+            let* _ <= log Log_Error (string_of_error err) #;
+            print_string ">>> "
         | _ => tt
         end) #;
         SomeE Recurse
@@ -41,7 +75,7 @@ Definition client_recv_thread (sockfd : file_descr) : optionE unit :=
 Definition client (host : string) (portno : port) : optionE unit :=
     (* Obtain username from user *)
     let* _ <= print_endline "Please enter a username (length 1-32, no spaces)" #;
-    let username_string := read_line tt in
+    username_string <- read_line tt ;;
     uname <- new_username username_string ;;
     (* Create a TCP socket to server *)
     let socket_fd := socket PF_INET SOCK_STREAM 0 in
@@ -67,7 +101,7 @@ Definition client (host : string) (portno : port) : optionE unit :=
     (* Display server messages *)
     recv_thread <- create file_descr (optionE unit) client_recv_thread socket_fd ;;
     let* _ <= join input_thread #;
-    let* _ <= join recv_thread #;
+    (* let* _ <= join recv_thread #; *)
     let* _ <= log Log_Info "Closing connection to server" #;
     let* _ <= close socket_fd #;
     return tt.
